Finish proof of size_of swap lemma

examples/cost/size_ofPropsScript.sml
@@ -6,6 +6,56 @@ open preamble dataSemTheory dataPropsTheory;
 
 val _ = new_theory "size_ofProps";
 
+Theorem delete_mk_BN:
+  (delete 0 (mk_BN t1 t2) = mk_BN t1 t2) ∧
+  (k ≠ 0 ⇒ delete k (mk_BN t1 t2) = delete k (BN t1 t2))
+Proof
+  Cases_on ‘t1’ \\ Cases_on ‘t2’ \\ fs [mk_BN_def]
+  \\ fs [delete_def,mk_BN_def]
+QED
+
+Theorem delete_mk_BS:
+  (delete 0 (mk_BS t1 s t2) = mk_BN t1 t2) ∧
+  (k ≠ 0 ⇒ delete k (mk_BS t1 s t2) = delete k (BS t1 s t2))
+Proof
+  Cases_on ‘t1’ \\ Cases_on ‘t2’ \\ fs [mk_BS_def]
+  \\ fs [delete_def,mk_BS_def,mk_BN_def]
+QED
+
+Triviality DIV_2_lemma:
+  n DIV 2 = m DIV 2 ∧ EVEN m = EVEN n ⇒ m = n
+Proof
+  rw []
+  \\ ‘0 < 2n’ by fs [] \\ drule DIVISION
+  \\ fs [EVEN_MOD2]
+  \\ disch_then (fn th => once_rewrite_tac [th]) \\ fs []
+  \\ Cases_on ‘m MOD 2 = 0’ \\ fs []
+  \\ ‘n MOD 2 < 2’ by fs [MOD_LESS]
+  \\ ‘m MOD 2 < 2’ by fs [MOD_LESS]
+  \\ decide_tac
+QED
+
+Theorem delete_delete:
+  ∀f n k.
+    delete n (delete k f) =
+    if n = k then delete n f else delete k (delete n f)
+Proof
+  Induct \\ fs [delete_def]
+  \\ rw [] \\ fs [delete_def]
+  \\ simp [delete_mk_BN,delete_mk_BS]
+  \\ rpt (qpat_x_assum ‘∀x. _’ (mp_tac o GSYM)) \\ rw []
+  \\ fs [delete_def]
+  \\ rpt (qpat_x_assum ‘∀x. _’ (fn th => simp [Once (GSYM th)])) \\ rw []
+  \\ rpt (rename [‘kk ≠ 0’] \\ Cases_on ‘kk’ \\ fs [])
+  \\ drule DIV_2_lemma \\ fs [EVEN]
+QED
+
+Theorem size_zero_empty:
+  ∀x. size x = 0 ⇔ domain x = EMPTY
+Proof
+  Induct \\ fs [size_def]
+QED
+
 Definition sane_timestamps_def:
   sane_timestamps l =
   ∀ts tag bl tag' bl'.
@@ -21,6 +71,12 @@ Definition all_blocks_def[simp]:
 Termination
   WF_REL_TAC ‘measure v1_size’
 End
+
+Theorem all_blocks_append:
+  ∀xs ys. all_blocks (xs ++ ys) = all_blocks xs ++ all_blocks ys
+Proof
+  Induct \\ fs [] \\ Cases \\ fs []
+QED
 
 Theorem size_of_cons:
   size_of lims (x::xs) refs seen =
@@ -43,38 +99,575 @@ Proof
   \\ once_rewrite_tac [size_of_cons] \\ fs [UNCURRY]
 QED
 
-Theorem size_of_refs_shirnk:
-  size_of lims ts refs seen = (n,refs1,seen1) ∧ refs ≠ refs1 ⇒
-  size refs1 < size refs
+Theorem size_of_refs_subspt:
+  ∀lims ts refs seen n refs1 seen1.
+    size_of lims ts refs seen = (n,refs1,seen1) ⇒ subspt refs1 refs
 Proof
-  cheat
+  ho_match_mp_tac size_of_ind \\ fs [size_of_def] \\ rw []
+  THEN1
+   (‘∃w. size_of lims (y::ys) refs seen = w’ by fs []
+    \\ PairCases_on ‘w’ \\ fs []
+    \\ ‘∃v. size_of lims [x] w1 w2 = v’ by fs []
+    \\ PairCases_on ‘v’ \\ fs [] \\ rveq  \\ fs []
+    \\ imp_res_tac subspt_trans \\ fs [])
+  THEN1
+   (fs [AllCaseEqs()]
+    THEN1
+     (‘∃w. size_of lims vs (delete r refs) seen = w’ by fs []
+      \\ PairCases_on ‘w’ \\ fs [] \\ fs [subspt_lookup,lookup_delete])
+    \\ rveq \\ fs [] \\ fs [subspt_lookup,lookup_delete])
+  \\ ‘∃w. size_of lims (v20::v21) refs (insert ts () seen) = w’ by fs []
+  \\ PairCases_on ‘w’ \\ fs []
+QED
+
+Theorem size_of_refs_size:
+  ∀lims ts refs seen n refs1 seen1.
+    size_of lims ts refs seen = (n,refs1,seen1) ⇒ size refs1 ≤ size refs
+Proof
+  ho_match_mp_tac size_of_ind \\ fs [size_of_def] \\ rw []
+  THEN1
+   (‘∃w. size_of lims (y::ys) refs seen = w’ by fs []
+    \\ PairCases_on ‘w’ \\ fs []
+    \\ ‘∃v. size_of lims [x] w1 w2 = v’ by fs []
+    \\ PairCases_on ‘v’ \\ fs [] \\ rveq  \\ fs [])
+  THEN1
+   (fs [AllCaseEqs()]
+    THEN1
+     (‘∃w. size_of lims vs (delete r refs) seen = w’ by fs []
+      \\ PairCases_on ‘w’ \\ fs [] \\ fs [subspt_lookup,lookup_delete]
+      \\ match_mp_tac LESS_EQ_TRANS \\ asm_exists_tac \\ fs []
+      \\ fs [size_delete])
+    \\ rveq \\ fs [] \\ fs [subspt_lookup,lookup_delete]
+    \\ fs [size_delete])
+  \\ ‘∃w. size_of lims (v20::v21) refs (insert ts () seen) = w’ by fs []
+  \\ PairCases_on ‘w’ \\ fs []
+QED
+
+Theorem size_of_refs_shirnk:
+  ∀lims ts refs seen n refs1 seen1.
+    size_of lims ts refs seen = (n,refs1,seen1) ∧ refs ≠ refs1 ⇒
+    size refs1 < size refs
+Proof
+  ho_match_mp_tac size_of_ind \\ fs [size_of_def] \\ rw []
+  THEN1
+   (‘∃w. size_of lims (y::ys) refs seen = w’ by fs []
+    \\ PairCases_on ‘w’ \\ fs []
+    \\ ‘∃v. size_of lims [x] w1 w2 = v’ by fs []
+    \\ PairCases_on ‘v’ \\ fs [] \\ rveq  \\ fs []
+    \\ imp_res_tac subspt_trans \\ fs []
+    \\ Cases_on ‘w1 = refs’ \\ fs []
+    \\ imp_res_tac size_of_refs_size
+    \\ fs [])
+  THEN1
+   (fs [AllCaseEqs()]
+    THEN1
+     (‘∃w. size_of lims vs (delete r refs) seen = w’ by fs []
+      \\ PairCases_on ‘w’ \\ fs [] \\ fs [subspt_lookup,lookup_delete]
+      \\ rveq \\ imp_res_tac size_of_refs_size
+      \\ match_mp_tac LESS_EQ_LESS_TRANS
+      \\ asm_exists_tac \\ fs []
+      \\ imp_res_tac lookup_zero \\ fs [size_delete])
+    \\ rveq \\ fs [] \\ fs [subspt_lookup,lookup_delete]
+    \\ imp_res_tac lookup_zero \\ fs [size_delete])
+  \\ ‘∃w. size_of lims (v20::v21) refs (insert ts () seen) = w’ by fs []
+  \\ PairCases_on ‘w’ \\ fs []
+QED
+
+Theorem size_of_refs_pres:
+  ∀x1 lims xs refs1 seen1 n refs2 seen2.
+    size_of lims xs refs1 seen1 = (n,refs2,seen2) ∧
+    lookup x1 refs1 = NONE ⇒
+    lookup x1 refs2 = NONE
+Proof
+  gen_tac \\ ho_match_mp_tac size_of_ind \\ fs [size_of_def] \\ rw []
+  THEN1
+   (‘∃w. size_of lims (y::ys) refs1 seen1 = w’ by fs []
+    \\ PairCases_on ‘w’ \\ fs []
+    \\ ‘∃v. size_of lims [x] w1 w2 = v’ by fs []
+    \\ PairCases_on ‘v’ \\ fs [] \\ rveq  \\ fs [])
+  THEN1
+   (fs [AllCaseEqs()] \\ rveq \\ fs []
+    THEN1
+     (‘∃w. size_of lims vs (delete r refs1) seen1 = w’ by fs []
+      \\ PairCases_on ‘w’ \\ fs [] \\ fs [subspt_lookup,lookup_delete])
+    \\ rveq \\ fs [] \\ fs [subspt_lookup,lookup_delete])
+  \\ ‘∃w. size_of lims (v20::v21) refs1 (insert ts () seen1) = w’ by fs []
+  \\ PairCases_on ‘w’ \\ fs []
+QED
+
+Theorem size_of_refs_ignored:
+  ∀lims xs refs1 seen1 n refs2 seen2 r x.
+    size_of lims xs refs1 seen1 = (n,refs2,seen2) ∧
+    lookup r refs2 = SOME x ⇒
+    size_of lims xs (delete r refs1) seen1 = (n,delete r refs2,seen2) ∧
+    lookup r refs1 = SOME x
+Proof
+  ho_match_mp_tac size_of_ind \\ fs [size_of_def]
+  \\ rpt conj_tac \\ rpt gen_tac \\ strip_tac \\ rpt gen_tac \\ strip_tac
+  THEN1
+   (‘∃w. size_of lims (y::ys) refs1 seen1 = w’ by fs []
+    \\ PairCases_on ‘w’ \\ fs []
+    \\ ‘∃v. size_of lims [x] w1 w2 = v’ by fs []
+    \\ PairCases_on ‘v’ \\ fs [] \\ rveq  \\ fs []
+    \\ res_tac \\ fs [])
+  THEN1
+   (fs [AllCaseEqs()] \\ rveq \\ fs [lookup_delete]
+    THEN1
+     (‘∃w. size_of lims vs (delete r refs1) seen1 = w’ by fs []
+      \\ PairCases_on ‘w’ \\ fs [] \\ fs [subspt_lookup,lookup_delete]
+      \\ rveq \\ fs [] \\ res_tac \\ fs []
+      \\ simp [Once delete_delete])
+    \\ simp [Once delete_delete])
+  \\ fs [AllCaseEqs()]
+  \\ ‘∃w. size_of lims (v20::v21) refs1 (insert ts () seen1) = w’ by fs []
+  \\ PairCases_on ‘w’ \\ fs []
 QED
 
 Theorem size_of_seen_pres:
-  size_of lims ys refs seen1 = (q0,q1,seen2) ∧
-  IS_SOME (lookup x1 seen1) ⇒
-  IS_SOME (lookup x1 seen2)
+  ∀lims xs refs seen1 n refs2 seen2.
+    size_of lims xs refs seen1 = (n,refs2,seen2) ⇒ subspt seen1 seen2
 Proof
-  cheat
+  ho_match_mp_tac size_of_ind \\ fs [size_of_def]
+  \\ rpt conj_tac \\ rpt gen_tac \\ strip_tac \\ rpt gen_tac \\ strip_tac
+  THEN1
+   (‘∃w. size_of lims (y::ys) refs seen1 = w’ by fs []
+    \\ PairCases_on ‘w’ \\ fs []
+    \\ ‘∃v. size_of lims [x] w1 w2 = v’ by fs []
+    \\ PairCases_on ‘v’ \\ fs [] \\ rveq  \\ fs []
+    \\ imp_res_tac subspt_trans)
+  THEN1
+   (fs [AllCaseEqs()] \\ rveq \\ fs [lookup_delete]
+    \\ ‘∃w. size_of lims vs (delete r refs) seen1 = w’ by fs []
+    \\ PairCases_on ‘w’ \\ fs [] \\ fs [subspt_lookup,lookup_delete])
+  \\ fs [AllCaseEqs()]
+  \\ ‘∃w. size_of lims (v20::v21) refs (insert ts () seen1) = w’ by fs []
+  \\ PairCases_on ‘w’ \\ fs []
+  \\ fs [subspt_lookup,lookup_insert]
 QED
 
 Theorem size_of_seen_ignored:
-  size_of lims ys refs seen1 = (q0,q1,seen2) ∧
-  lookup x1 seen1 = NONE ∧
-  lookup x1 seen2 = NONE ⇒
-  size_of lims ys refs (insert x1 () seen1) = (q0,q1,insert x1 () seen2)
+  ∀x1 lims xs refs seen1 n refs2 seen2.
+    size_of lims xs refs seen1 = (n,refs2,seen2) ∧
+    lookup x1 seen2 = NONE ⇒
+    size_of lims xs refs (insert x1 () seen1) = (n,refs2,insert x1 () seen2) ∧
+    lookup x1 seen1 = NONE
 Proof
-  cheat
+  gen_tac \\ ho_match_mp_tac size_of_ind \\ fs [size_of_def]
+  \\ rpt conj_tac \\ rpt gen_tac \\ strip_tac \\ rpt gen_tac \\ strip_tac
+  THEN1
+   (‘∃w. size_of lims (y::ys) refs seen1 = w’ by fs []
+    \\ PairCases_on ‘w’ \\ fs []
+    \\ ‘∃v. size_of lims [x] w1 w2 = v’ by fs []
+    \\ PairCases_on ‘v’ \\ fs [] \\ rveq  \\ fs [])
+  THEN1
+   (fs [AllCaseEqs()] \\ rveq \\ fs [lookup_delete]
+    \\ ‘∃w. size_of lims vs (delete r refs) seen1 = w’ by fs []
+    \\ PairCases_on ‘w’ \\ fs [] \\ fs [subspt_lookup,lookup_delete])
+  \\ Cases_on ‘ts = x1’ \\ fs []
+  THEN1
+   (Cases_on ‘lookup x1 seen1’ \\ fs [] \\ rveq \\ fs []
+    \\ ‘∃w. size_of lims (v20::v21) refs (insert ts () seen1) = w’ by fs []
+    \\ PairCases_on ‘w’ \\ fs [])
+  \\ fs [lookup_insert]
+  \\ simp [Once insert_insert]
+  \\ Cases_on ‘lookup ts seen1’ \\ fs []
+  \\ ‘∃w. size_of lims (v20::v21) refs (insert ts () seen1) = w’ by fs []
+  \\ PairCases_on ‘w’ \\ fs []
 QED
 
-(* TODO: the refs also need have sane_timestamps, but that can wait until later *)
+Theorem v_size_append:
+  ∀xs ys. v1_size (xs ++ ys) = v1_size xs + v1_size ys
+Proof
+  Induct \\ fs [v_size_def]
+QED
+
+Definition refs_in_def:
+  refs_in refs bs ⇔
+    ∀n vals. lookup n refs = SOME (ValueArray vals) ⇒
+             set (all_blocks vals) SUBSET set bs
+End
+
+Theorem size_of_lemma:
+  ∀refs qs seen1 k0 refs1 seen2.
+    size_of lims qs refs seen1 = (k0,refs1,seen2) ∧ bb ≠ [] ∧
+    (∀refs' xs ys zs seen.
+       (if refs ≠ refs' then size refs' < size refs else
+          v1_size (xs ++ ys ++ zs) ≤ v1_size (bb ++ qs)) ∧
+       sane_timestamps bs ∧ refs_in refs' bs ∧
+       set (all_blocks xs ++ all_blocks ys ++ all_blocks zs) SUBSET set bs ⇒
+       size_of lims (xs ++ ys ++ zs) refs' seen =
+       size_of lims (ys ++ xs ++ zs) refs' seen) ∧
+    lookup x1 seen1 = NONE ∧ IS_SOME (lookup x1 seen2) ∧
+    sane_timestamps bs ∧ refs_in refs bs ∧
+    MEM (Block x1 x2 bb) bs ∧
+    set (all_blocks bb ++ all_blocks qs) SUBSET set bs ⇒
+    size_of lims qs refs seen1 =
+      let (n1,refs1,seen1) = size_of lims (bb ++ qs) refs (insert x1 () seen1) in
+        (n1 + LENGTH bb + 1,refs1,seen1)
+Proof
+  gen_tac
+  \\ completeInduct_on ‘size refs’
+  \\ simp [Once PULL_FORALL]
+  \\ completeInduct_on ‘v1_size qs’
+  \\ rpt strip_tac \\ rpt var_eq_tac
+  \\ Cases_on ‘qs’ \\ fs []
+  THEN1 (fs [size_of_def] \\ rw [] \\ fs [] \\ rfs [])
+  \\ Cases_on ‘t = []’
+  THEN1
+   (rveq
+    \\ reverse (Cases_on ‘h’) \\ fs [size_of_def,AllCaseEqs()]
+    \\ rveq \\ fs [] \\ rfs []
+    THEN1
+     (rewrite_tac [size_of_append,size_of_def] \\ simp []
+      \\ Cases_on ‘size_of lims vs (delete n refs) seen1’ \\ fs []
+      \\ PairCases_on ‘r’ \\ fs [] \\ rveq
+      \\ last_x_assum (qspec_then ‘size (delete n refs)’ mp_tac)
+      \\ impl_tac
+      THEN1 (fs [size_delete] \\ imp_res_tac lookup_zero \\ fs [])
+      \\ disch_then (qspec_then ‘delete n refs’ mp_tac)
+      \\ rewrite_tac []
+      \\ disch_then (qspecl_then [‘vs’,‘seen1’] mp_tac)
+      \\ simp []
+      \\ reverse impl_tac
+      THEN1 (fs [size_of_append] \\ fs [UNCURRY])
+      \\ rpt strip_tac
+      THEN1
+       (first_x_assum match_mp_tac \\ fs []
+        \\ Cases_on ‘refs'' = delete n refs’ \\ rveq \\ fs []
+        THEN1
+         (rw [] THEN1 (fs [size_delete] \\ imp_res_tac lookup_zero \\ fs [])
+          \\ rpt (qpat_x_assum ‘lookup _ _ = _’ mp_tac)
+          \\ pop_assum (fn th => once_rewrite_tac [th])
+          \\ simp [lookup_delete])
+        \\ rw [] \\ fs [size_delete] \\ rfs [])
+      \\ fs [refs_in_def,lookup_delete] \\ metis_tac [])
+    \\ Cases_on ‘l’ \\ fs [size_of_def,CaseEq"bool"]
+    \\ rveq \\ fs [] \\ rfs []
+    \\ ‘∃rr. size_of lims (h::t) refs (insert n0 () seen1) = rr’ by fs []
+    \\ PairCases_on ‘rr’ \\ fs [] \\ rveq \\ fs []
+    \\ asm_rewrite_tac [size_of_append,size_of_def,lookup_insert]
+    \\ rename [‘if t1 = t2 then SOME () else NONE’]
+    \\ Cases_on ‘t1 = t2’ \\ fs []
+    THEN1 (‘bb = h::t’by (fs [sane_timestamps_def] \\ res_tac \\ fs []) \\ fs [])
+    \\ first_x_assum (qspec_then ‘v1_size (h::t)’ mp_tac)
+    \\ impl_tac THEN1 fs [v_size_def,v_size_append]
+    \\ disch_then (qspec_then ‘h::t’ mp_tac)
+    \\ rewrite_tac []
+    \\ disch_then (qspec_then ‘refs’ mp_tac)
+    \\ rewrite_tac []
+    \\ disch_then (qspecl_then [‘(insert t1 () seen1)’] mp_tac) \\ simp []
+    \\ impl_tac THEN1
+     (fs [lookup_insert] \\ rw []
+      \\ first_x_assum match_mp_tac
+      \\ fs [v_size_def,v_size_append])
+    \\ strip_tac
+    \\ once_rewrite_tac [insert_insert]
+    \\ simp []
+    \\ ‘∃w. size_of lims (h::t) refs (insert t2 () (insert t1 () seen1)) = w’ by fs []
+    \\ PairCases_on ‘w’ \\ fs []
+    \\ ntac 4 (pop_assum mp_tac)
+    \\ rewrite_tac [size_of_append]
+    \\ rpt strip_tac \\ fs [] \\ rfs []
+    \\ ‘∃v. size_of lims bb w1 w2 = v’ by fs []
+    \\ PairCases_on ‘v’ \\ fs [])
+  \\ ‘size_of lims ([h] ++ t) refs seen1 = (k0,refs1,seen2)’ by fs []
+  \\ pop_assum mp_tac
+  \\ simp [Once size_of_append]
+  \\ strip_tac
+  \\ ‘size_of lims (bb ++ h::t) refs = size_of lims (bb ++ ([h] ++ t)) refs’
+      by rewrite_tac [APPEND]
+  \\ asm_rewrite_tac [] \\ rewrite_tac [size_of_append]
+  \\ ‘∃v. size_of lims t refs seen1 = v’ by fs []
+  \\ PairCases_on ‘v’ \\ fs []
+  \\ rename [‘_ = (n7,refs7,seen7)’]
+  \\ ‘∃w. size_of lims [h] refs7 seen7 = w’ by fs []
+  \\ PairCases_on ‘w’ \\ fs [] \\ rveq
+  \\ reverse (Cases_on ‘IS_SOME (lookup x1 seen7)’) \\ fs []
+  THEN1
+   (qpat_x_assum ‘size_of lims t refs seen1 = (n7,refs7,seen7)’ assume_tac
+    \\ drule size_of_seen_ignored
+    \\ disch_then drule
+    \\ asm_rewrite_tac []
+    \\ strip_tac \\ simp []
+    \\ Cases_on ‘refs7 = refs’ \\ fs []
+    THEN1
+     (first_x_assum (qspec_then ‘v1_size [h]’ mp_tac)
+      \\ impl_tac THEN1 (Cases_on ‘t’ \\ fs [v_size_def])
+      \\ disch_then (qspec_then ‘[h]’ mp_tac) \\ rewrite_tac []
+      \\ disch_then (qspec_then ‘refs’ mp_tac) \\ rewrite_tac []
+      \\ disch_then (qspec_then ‘seen7’ mp_tac) \\ simp []
+      \\ impl_tac
+      THEN1
+       (reverse conj_tac THEN1 (Cases_on ‘h’ \\ fs [])
+        \\ rveq \\ rpt strip_tac
+        \\ first_x_assum match_mp_tac \\ fs []
+        \\ rw [] \\ fs [] \\ fs [v_size_def,v_size_append])
+      \\ rewrite_tac [size_of_append]
+      \\ fs [UNCURRY])
+    \\ last_x_assum (qspec_then ‘size refs7’ mp_tac)
+    \\ impl_keep_tac
+    THEN1
+     (match_mp_tac (GEN_ALL size_of_refs_shirnk)
+      \\ asm_exists_tac \\ fs [])
+    \\ disch_then (qspec_then ‘refs7’ mp_tac) \\ rewrite_tac []
+    \\ disch_then drule
+    \\ reverse impl_tac
+    THEN1 (rewrite_tac [size_of_append] \\ fs [UNCURRY])
+    \\ fs []
+    \\ reverse (rpt strip_tac)
+    THEN1 (Cases_on ‘h’ \\ fs [])
+    THEN1
+     (imp_res_tac size_of_refs_subspt
+      \\ fs [refs_in_def,subspt_lookup]
+      \\ metis_tac [])
+    \\ first_x_assum match_mp_tac \\ fs []
+    \\ reverse IF_CASES_TAC
+    THEN1 (fs [] \\ rfs [])
+    \\ match_mp_tac LESS_EQ_LESS_TRANS
+    \\ qexists_tac ‘size refs7’ \\ fs []
+    \\ Cases_on ‘refs'' = refs7’ \\ fs [])
+  \\ first_x_assum (qspec_then ‘v1_size t’ mp_tac)
+  \\ impl_tac THEN1 (Cases_on ‘t’ \\ fs [v_size_def])
+  \\ disch_then (qspec_then ‘t’ mp_tac) \\ rewrite_tac []
+  \\ disch_then (qspec_then ‘refs’ mp_tac) \\ rewrite_tac []
+  \\ disch_then (qspec_then ‘seen1’ mp_tac) \\ simp []
+  \\ impl_tac
+  THEN1
+   (reverse conj_tac THEN1 (Cases_on ‘h’ \\ fs [])
+    \\ rpt strip_tac
+    \\ first_x_assum match_mp_tac \\ fs []
+    \\ rw [] \\ fs [v_size_append,v_size_def])
+  \\ rewrite_tac [size_of_append]
+  \\ ‘∃v. size_of lims t refs (insert x1 () seen1) = v’ by fs []
+  \\ PairCases_on ‘v’ \\ fs []
+  \\ ‘∃w. size_of lims bb v1 v2 = w’ by fs []
+  \\ PairCases_on ‘w’ \\ fs []
+  \\ strip_tac \\ rveq \\ fs []
+  \\ qsuff_tac
+       ‘size_of lims ([h] ++ bb ++ []) v1 v2 =
+        size_of lims (bb ++ [h] ++ []) v1 v2’
+  THEN1 (rewrite_tac [APPEND_NIL] \\ rewrite_tac [size_of_append] \\ fs [UNCURRY])
+  \\ first_x_assum match_mp_tac \\ fs []
+  \\ reverse (rpt strip_tac)
+  THEN1 (Cases_on ‘h’ \\ fs [])
+  THEN1
+   (pop_assum kall_tac
+    \\ drule size_of_refs_subspt
+    \\ fs [subspt_lookup,refs_in_def] \\ metis_tac [])
+  \\ rw []
+  THEN1 metis_tac [size_of_refs_shirnk]
+  \\ fs [v_size_def,v_size_append]
+QED
+
+Definition array_vals_def:
+  array_vals (ValueArray vs) = vs ∧
+  array_vals _ = []
+End
+
+Definition array_len_def:
+  array_len lims (ValueArray vs) = LENGTH vs + 1 ∧
+  array_len lims (ByteArray _ b) = LENGTH b DIV (arch_size lims DIV 8) + 2
+End
+
+Triviality size_of_ref:
+  size_of lims [RefPtr r] refs seen =
+    case lookup r refs of
+    | NONE => (0,refs,seen)
+    | SOME x =>
+        let (n,refs',seen') = size_of lims (array_vals x) (delete r refs) seen in
+          (n + array_len lims x,refs',seen')
+Proof
+  fs [size_of_def]
+  \\ Cases_on ‘lookup r refs’ \\ fs []
+  \\ Cases_on ‘x’ \\ fs [size_of_def,array_vals_def,array_len_def]
+QED
+
+Theorem size_of_lemma_ref:
+  ∀refs qs r x seen1 k0 refs1 seen2.
+    size_of lims qs refs seen1 = (k0,refs1,seen2) ∧
+    (∀refs' xs ys zs seen.
+       (if refs ≠ refs' then size refs' < size refs else
+          v1_size (xs ++ ys ++ zs) ≤ v1_size qs) ∧
+       sane_timestamps bs ∧ refs_in refs' bs ∧
+       set (all_blocks xs ++ all_blocks ys ++ all_blocks zs) SUBSET set bs ⇒
+       size_of lims (xs ++ ys ++ zs) refs' seen =
+       size_of lims (ys ++ xs ++ zs) refs' seen) ∧
+    lookup r refs = SOME x ∧ lookup r refs1 = NONE ∧
+    sane_timestamps bs ∧ refs_in refs bs ∧
+    set (all_blocks qs) SUBSET set bs ⇒
+    size_of lims qs refs seen1 =
+      let (n1,refs1,seen1) = size_of lims (array_vals x ++ qs) (delete r refs) seen1 in
+        (n1 + array_len lims x,refs1,seen1)
+Proof
+  gen_tac
+  \\ completeInduct_on ‘size refs’
+  \\ simp [Once PULL_FORALL]
+  \\ completeInduct_on ‘v1_size qs’
+  \\ rpt strip_tac \\ rpt var_eq_tac
+  \\ Cases_on ‘qs’ \\ fs []
+  THEN1 (fs [size_of_def] \\ rw [] \\ fs [] \\ rfs [])
+  \\ Cases_on ‘t = []’
+  THEN1
+   (rveq \\ Cases_on ‘h’ \\ fs [size_of_ref]
+    \\ fs [size_of_def,AllCaseEqs()]
+    \\ TRY (Cases_on ‘l’ \\ fs [size_of_def])
+    \\ rveq \\ fs [] \\ rfs []
+    THEN1
+     (Cases_on ‘IS_SOME (lookup n0 seen1)’ \\ fs [] \\ rfs []
+      \\ ‘∃b. size_of lims (h::t) refs (insert n0 () seen1) = b’ by fs []
+      \\ PairCases_on ‘b’ \\ fs [] \\ rveq
+      \\ first_x_assum (qspec_then ‘v1_size (h::t)’ mp_tac)
+      \\ impl_tac THEN1 fs [v_size_def]
+      \\ disch_then (qspec_then ‘h::t’ mp_tac)
+      \\ rewrite_tac []
+      \\ disch_then (qspecl_then [‘refs’] mp_tac) \\ simp []
+      \\ disch_then (qspecl_then [‘r’,‘x’,‘insert n0 () seen1’] mp_tac) \\ simp []
+      \\ impl_tac
+      THEN1
+       (rpt strip_tac
+        \\ first_x_assum match_mp_tac \\ fs []
+        \\ rw [] \\ fs [v_size_def])
+      \\ rewrite_tac [size_of_append,size_of_def]
+      \\ fs [UNCURRY])
+    \\ Cases_on ‘n = r’ \\ fs [] \\ rveq
+    THEN1
+     (rewrite_tac [size_of_append,size_of_def,lookup_delete] \\ fs []
+      \\ fs [UNCURRY])
+    \\ ‘∃rr. size_of lims (array_vals x') (delete n refs) seen1 = rr’ by fs []
+    \\ PairCases_on ‘rr’ \\ fs [] \\ rveq \\ fs []
+    \\ asm_rewrite_tac [size_of_append,size_of_ref,lookup_insert,lookup_delete]
+    \\ simp []
+    \\ last_x_assum (qspec_then ‘size (delete n refs)’ mp_tac)
+    \\ impl_tac THEN1 (imp_res_tac lookup_zero \\ fs [size_delete])
+    \\ disch_then (qspec_then ‘delete n refs’ mp_tac)
+    \\ rewrite_tac []
+    \\ disch_then drule
+    \\ disch_then (qspecl_then [‘r’,‘x’] mp_tac) \\ simp []
+    \\ impl_tac
+    THEN1
+     (fs [lookup_delete] \\ reverse (rw [])
+      THEN1
+       (fs [refs_in_def] \\ res_tac
+        \\ Cases_on ‘x'’ \\ fs [array_vals_def] \\ metis_tac [])
+      THEN1 (fs [refs_in_def,lookup_delete] \\ metis_tac [])
+      \\ first_x_assum match_mp_tac \\ fs []
+      \\ rw [] \\ fs []
+      THEN1 (imp_res_tac lookup_zero \\ fs [size_delete])
+      THEN1 (‘lookup n refs = lookup n (delete n refs)’ by metis_tac []
+        \\ fs [lookup_delete] \\ rfs [])
+      THEN1
+       (match_mp_tac LESS_TRANS \\ asm_exists_tac \\ fs []
+        \\ imp_res_tac lookup_zero \\ fs [size_delete])
+      \\ imp_res_tac lookup_zero \\ fs [size_delete] \\ rfs [])
+    \\ simp [Once delete_delete]
+    \\ rewrite_tac [size_of_append]
+    \\ fs [UNCURRY])
+  \\ ‘size_of lims ([h] ++ t) refs seen1 = (k0,refs1,seen2)’ by fs []
+  \\ pop_assum mp_tac
+  \\ simp [Once size_of_append]
+  \\ strip_tac
+  \\ ‘size_of lims (array_vals x ++ h::t) =
+      size_of lims (array_vals x ++ ([h] ++ t))’
+        by rewrite_tac [APPEND]
+  \\ asm_rewrite_tac [] \\ rewrite_tac [size_of_append]
+  \\ ‘∃v. size_of lims t refs seen1 = v’ by fs []
+  \\ PairCases_on ‘v’ \\ fs []
+  \\ rename [‘_ = (n7,refs7,seen7)’]
+  \\ ‘∃w. size_of lims [h] refs7 seen7 = w’ by fs []
+  \\ PairCases_on ‘w’ \\ fs [] \\ rveq
+  \\ reverse (Cases_on ‘lookup r refs7’) \\ fs []
+  THEN1
+   (qpat_x_assum ‘size_of lims t refs seen1 = (n7,refs7,seen7)’ assume_tac
+    \\ drule size_of_refs_ignored
+    \\ disch_then drule
+    \\ asm_rewrite_tac []
+    \\ strip_tac \\ simp []
+    \\ fs [] \\ rveq
+    \\ Cases_on ‘refs7 = refs’ \\ fs []
+    THEN1
+     (first_x_assum (qspec_then ‘v1_size [h]’ mp_tac)
+      \\ impl_tac THEN1 (Cases_on ‘t’ \\ fs [v_size_def])
+      \\ disch_then (qspec_then ‘[h]’ mp_tac) \\ rewrite_tac []
+      \\ disch_then (qspec_then ‘refs’ mp_tac) \\ rewrite_tac []
+      \\ disch_then (qspecl_then [‘r’,‘x’,‘seen7’] mp_tac) \\ simp []
+      \\ impl_tac
+      THEN1
+       (reverse conj_tac THEN1 (Cases_on ‘h’ \\ fs [])
+        \\ rveq \\ rpt strip_tac
+        \\ first_x_assum match_mp_tac \\ fs []
+        \\ rw [] \\ fs [] \\ fs [v_size_def,v_size_append])
+      \\ rewrite_tac [size_of_append]
+      \\ fs [UNCURRY])
+    \\ last_x_assum (qspec_then ‘size refs7’ mp_tac)
+    \\ impl_keep_tac
+    THEN1
+     (match_mp_tac (GEN_ALL size_of_refs_shirnk)
+      \\ asm_exists_tac \\ fs [])
+    \\ disch_then (qspec_then ‘refs7’ mp_tac) \\ rewrite_tac []
+    \\ disch_then drule
+    \\ disch_then (qspecl_then [‘r’,‘x’] mp_tac) \\ rewrite_tac []
+    \\ reverse impl_tac
+    THEN1 (rewrite_tac [size_of_append] \\ fs [UNCURRY])
+    \\ fs []
+    \\ reverse (rpt strip_tac)
+    THEN1 (Cases_on ‘h’ \\ fs [])
+    THEN1
+     (imp_res_tac size_of_refs_subspt
+      \\ fs [refs_in_def,subspt_lookup]
+      \\ metis_tac [])
+    \\ first_x_assum match_mp_tac \\ fs []
+    \\ reverse IF_CASES_TAC
+    THEN1 (fs [] \\ rfs [])
+    \\ match_mp_tac LESS_EQ_LESS_TRANS
+    \\ qexists_tac ‘size refs7’ \\ fs []
+    \\ Cases_on ‘refs'' = refs7’ \\ fs [])
+  \\ first_x_assum (qspec_then ‘v1_size t’ mp_tac)
+  \\ impl_tac THEN1 (Cases_on ‘t’ \\ fs [v_size_def])
+  \\ disch_then (qspec_then ‘t’ mp_tac) \\ rewrite_tac []
+  \\ disch_then (qspec_then ‘refs’ mp_tac) \\ rewrite_tac []
+  \\ disch_then (qspecl_then [‘r’,‘x’,‘seen1’] mp_tac) \\ simp []
+  \\ impl_tac
+  THEN1
+   (reverse conj_tac THEN1 (Cases_on ‘h’ \\ fs [])
+    \\ rpt strip_tac
+    \\ first_x_assum match_mp_tac \\ fs []
+    \\ rw [] \\ fs [v_size_append,v_size_def])
+  \\ rewrite_tac [size_of_append]
+  \\ ‘∃v. size_of lims t (delete r refs) seen1 = v’ by fs []
+  \\ PairCases_on ‘v’ \\ fs []
+  \\ ‘∃w. size_of lims (array_vals x) v1 v2 = w’ by fs []
+  \\ PairCases_on ‘w’ \\ fs []
+  \\ strip_tac \\ rveq \\ fs []
+  \\ qsuff_tac
+       ‘size_of lims ([h] ++ array_vals x ++ []) v1 v2 =
+        size_of lims (array_vals x ++ [h] ++ []) v1 v2’
+  THEN1 (rewrite_tac [APPEND_NIL] \\ rewrite_tac [size_of_append] \\ fs [UNCURRY])
+  \\ first_x_assum match_mp_tac \\ fs []
+  \\ reverse (rpt strip_tac)
+  THEN1 (Cases_on ‘x’ \\ fs [array_vals_def,refs_in_def] \\ metis_tac [])
+  THEN1 (Cases_on ‘h’ \\ fs [])
+  THEN1
+   (pop_assum kall_tac
+    \\ drule size_of_refs_subspt
+    \\ fs [subspt_lookup,refs_in_def,lookup_delete] \\ metis_tac [])
+  \\ pop_assum kall_tac
+  \\ drule size_of_refs_size
+  \\ strip_tac
+  \\ ‘size (delete r refs) < size refs’ by
+        (imp_res_tac lookup_zero \\ fs [size_delete])
+  \\ ‘size v1 < size refs’ by fs []
+  \\ IF_CASES_TAC \\ fs []
+QED
+
 Theorem size_of_swap:
-  ∀lims refs xs ys zs seen.
-    sane_timestamps (all_blocks xs ++ all_blocks ys ++ all_blocks zs) ⇒
+  ∀bs lims refs xs ys zs seen.
+    sane_timestamps bs ∧ refs_in refs bs ∧
+    set (all_blocks xs ++ all_blocks ys ++ all_blocks zs) SUBSET set bs ⇒
     size_of lims (xs ++ ys ++ zs) refs seen =
     size_of lims (ys ++ xs ++ zs) refs seen
 Proof
-  gen_tac \\ gen_tac
+  gen_tac \\ Cases_on ‘sane_timestamps bs’ \\ fs []
+  \\ gen_tac \\ gen_tac
   \\ completeInduct_on ‘size refs’
   \\ fs [PULL_FORALL]
   \\ completeInduct_on ‘v1_size (xs ++ ys ++ zs)’
@@ -95,9 +688,6 @@ Proof
     \\ fs [v_size_def]
     \\ fs [sane_timestamps_def,all_blocks_def]
     \\ rpt gen_tac
-    \\ disch_then assume_tac
-    \\ first_x_assum match_mp_tac
-    \\ qexists_tac ‘ts’
     \\ Cases_on ‘h’ \\ fs [])
   \\ qsuff_tac
      ‘size_of lims (h::ys ++ (t ++ zs)) refs seen =
@@ -116,12 +706,11 @@ Proof
    (rw [] \\ last_x_assum drule
     \\ disch_then (qspecl_then [‘[h]’,‘ys’,‘[]’] mp_tac) \\ fs []
     \\ disch_then match_mp_tac
-    \\ fs [sane_timestamps_def]
-    \\ rpt gen_tac
-    \\ disch_then assume_tac
-    \\ first_x_assum match_mp_tac
-    \\ qexists_tac ‘ts'’
-    \\ Cases_on ‘h’ \\ fs [] \\ metis_tac []) \\ fs []
+    \\ conj_tac
+    THEN1
+     (imp_res_tac size_of_refs_subspt
+      \\ fs [refs_in_def,subspt_lookup] \\ metis_tac [])
+    \\ Cases_on ‘h’ \\ fs []) \\ fs []
   \\ var_eq_tac
   \\ qsuff_tac ‘size_of lims ([h] ++ ys) refs seen1 =
                 size_of lims (ys ++ [h]) refs seen1’
@@ -129,7 +718,6 @@ Proof
   \\ Cases_on ‘h’
   \\ TRY (rename [‘Block x1 x2 x3’] \\ Cases_on ‘x3’)
   \\ TRY (rewrite_tac [size_of_append] \\ simp [size_of_def] \\ NO_TAC)
-
   (* only non-empty Block and RefPtr cases left *)
   THEN1
    (rewrite_tac [size_of_append] \\ simp [size_of_def]
@@ -137,24 +725,132 @@ Proof
     THEN1
      (‘∃q. size_of lims ys refs seen1 = q’ by fs []
       \\ PairCases_on ‘q’ \\ fs []
-      \\ imp_res_tac size_of_seen_pres \\ fs [])
+      \\ imp_res_tac size_of_seen_pres \\ fs []
+      \\ fs [subspt_lookup]
+      \\ Cases_on ‘lookup x1 seen1’ \\ fs [])
     \\ ‘∃q. size_of lims ys refs seen1 = q’ by fs []
     \\ PairCases_on ‘q’ \\ fs []
     \\ reverse IF_CASES_TAC \\ fs []
     THEN1
      (drule size_of_seen_ignored
       \\ disch_then drule \\ fs []
-      \\ cheat (* confusing but probably follows from IH *))
+      \\ strip_tac
+      \\ ‘∃w. size_of lims (h::t') q1 (insert x1 () q2) = w’ by fs []
+      \\ PairCases_on ‘w’ \\ fs []
+      \\ ‘∃v. size_of lims (h::t') refs (insert x1 () seen1) = v’ by fs []
+      \\ PairCases_on ‘v’ \\ fs []
+      \\ ‘∃x. size_of lims ys v1 v2 = x’ by fs []
+      \\ PairCases_on ‘x’ \\ fs []
+      \\ last_x_assum (qspecl_then [‘ys’,‘h::t'’,‘[]’,‘refs’,‘insert x1 () seen1’] mp_tac)
+      \\ impl_tac THEN1 fs [v_size_def,v_size_append]
+      \\ rewrite_tac [APPEND_NIL]
+      \\ asm_rewrite_tac [size_of_append] \\ fs [])
     \\ qsuff_tac ‘size_of lims ys refs seen1 =
        size_of lims (ys ++ [Block x1 x2 (h::t')]) refs seen1’
     THEN1
      (fs [] \\ disch_then kall_tac
       \\ simp [Once size_of_append]
       \\ fs [size_of_def])
+    \\ asm_rewrite_tac [size_of_append,size_of_def,EVAL “IS_SOME NONE”]
+    \\ drule size_of_lemma
+    \\ rename [‘Block x1 x2 (x3::x4)’]
+    \\ disch_then (qspecl_then [‘x2’,‘x1’,‘bs’,‘x3::x4’] mp_tac)
+    \\ impl_tac
+    THEN1
+     (fs [SUBSET_DEF] \\ rw [] \\ fs []
+      \\ first_x_assum match_mp_tac \\ fs []
+      \\ fs [v_size_append,v_size_def])
+    \\ first_assum (qspecl_then [‘x3::x4’,‘ys’,‘[]’,‘refs’,‘insert x1 () seen1’] mp_tac)
+    \\ impl_tac THEN1 fs [v_size_def,v_size_append]
+    \\ rewrite_tac [APPEND_NIL]
+    \\ rewrite_tac [size_of_append]
+    \\ fs [UNCURRY])
+  \\ rewrite_tac [size_of_append] \\ simp [size_of_def]
+  \\ rename [‘lookup r’]
+  \\ Cases_on ‘lookup r refs’ \\ fs []
+  THEN1
+   (‘∃q. size_of lims ys refs seen1 = q’ by fs []
+    \\ PairCases_on ‘q’ \\ fs []
+    \\ imp_res_tac size_of_refs_pres \\ fs [])
+  \\ ‘∃q. size_of lims ys refs seen1 = q’ by fs []
+  \\ PairCases_on ‘q’ \\ fs []
+  \\ reverse (Cases_on ‘lookup r q1’) \\ fs []
+  THEN1
+   (drule size_of_refs_ignored
+    \\ disch_then drule \\ fs []
+    \\ strip_tac \\ rveq
+    \\ Cases_on ‘x’ \\ fs []
+    \\ ‘∃w. size_of lims l (delete r q1) q2 = w’ by fs []
+    \\ PairCases_on ‘w’ \\ fs []
+    \\ ‘∃v. size_of lims l (delete r refs) seen1 = v’ by fs []
+    \\ PairCases_on ‘v’ \\ fs []
+    \\ ‘∃x. size_of lims ys v1 v2 = x’ by fs []
+    \\ PairCases_on ‘x’ \\ fs []
+    \\ first_x_assum (qspecl_then [‘delete r refs’,‘ys’,‘l’,‘[]’,‘seen1’] mp_tac)
+    \\ impl_tac THEN1
+     (fs [] \\ rpt strip_tac
+      THEN1 (imp_res_tac lookup_zero \\ fs [size_delete])
+      THEN1 (fs [refs_in_def,lookup_delete] \\ metis_tac [])
+      \\ fs [array_vals_def,refs_in_def] \\ res_tac)
+    \\ rewrite_tac [APPEND_NIL] \\ asm_rewrite_tac [size_of_append] \\ fs [])
+  \\ qsuff_tac ‘size_of lims ys refs seen1 =
+                size_of lims (ys ++ [RefPtr r]) refs seen1’
+  THEN1
+   (fs [] \\ disch_then kall_tac
+    \\ simp [Once size_of_append]
+    \\ fs [size_of_def])
+  \\ asm_rewrite_tac [size_of_append,size_of_def]
+  \\ drule size_of_lemma_ref
+  \\ disch_then (qspecl_then [‘bs’,‘r’] mp_tac) \\ simp []
+  \\ impl_tac
+  THEN1
+   (fs [SUBSET_DEF] \\ rw [] \\ fs []
+    \\ first_x_assum match_mp_tac \\ fs []
+    \\ fs [v_size_append,v_size_def])
+  \\ first_assum (qspecl_then [‘delete r refs’,‘array_vals x’,‘ys’,‘[]’,‘seen1’] mp_tac)
+  \\ impl_tac THEN1
+   (fs [] \\ rpt strip_tac
+    THEN1 (imp_res_tac lookup_zero \\ fs [size_delete])
+    THEN1 (fs [refs_in_def,lookup_delete] \\ metis_tac [])
+    \\ Cases_on ‘x’ \\ fs [array_vals_def,refs_in_def] \\ res_tac)
+  \\ rewrite_tac [APPEND_NIL]
+  \\ rewrite_tac [size_of_append]
+  \\ Cases_on ‘x’ \\ fs [array_vals_def,array_len_def]
+  \\ fs [size_of_def]
+  \\ fs [UNCURRY] \\ rw [] \\ fs []
+QED
 
-    \\ cheat (* could the IH save the day here?! *))
-
-  \\ cheat
+Theorem size_of_perm:
+  ∀xs ys lims bs refs seen.
+    PERM xs ys ∧ sane_timestamps bs ∧
+    refs_in refs bs ∧ set (all_blocks xs) ⊆ set bs ⇒
+    size_of lims xs refs seen =
+    size_of lims ys refs seen
+Proof
+  rewrite_tac [GSYM AND_IMP_INTRO]
+  \\ simp [GSYM PULL_FORALL,PERM_RTC]
+  \\ ho_match_mp_tac RTC_INDUCT \\ rw []
+  \\ match_mp_tac EQ_TRANS
+  \\ qexists_tac ‘size_of lims xs' refs seen’
+  \\ reverse conj_tac
+  THEN1
+   (fs [PULL_FORALL,AND_IMP_INTRO]
+    \\ first_x_assum match_mp_tac
+    \\ asm_exists_tac \\ fs []
+    \\ fs [PERM_SINGLE_SWAP_DEF]
+    \\ rveq \\ fs [all_blocks_append])
+  \\ qpat_x_assum ‘∀x. _’ kall_tac
+  \\ fs [PERM_SINGLE_SWAP_DEF]
+  \\ rveq \\ fs []
+  \\ rewrite_tac [GSYM APPEND_ASSOC]
+  \\ once_rewrite_tac [size_of_append]
+  \\ simp [] \\ AP_TERM_TAC
+  \\ qsuff_tac ‘size_of lims (x2 ++ x3 ++ []) refs seen =
+                size_of lims (x3 ++ x2 ++ []) refs seen’
+  THEN1 fs [APPEND_NIL]
+  \\ match_mp_tac size_of_swap
+  \\ asm_exists_tac \\ fs []
+  \\ fs [all_blocks_append]
 QED
 
 val _ = export_theory();
